theories/case_studies/multiuser_kvs/kvs_spec_addOrUpdate_safe.v
@@ -4,7 +4,7 @@ From griotte Require Import logrel rules.
 From griotte Require Import region_invariants_revocation wp_rules_interp interp_weakening.
 From griotte Require Import switcher_preamble switcher_spec_return.
 From griotte Require Import
-  switcher kvs kvs_preamble kvs_spec_getFullKey kvs_spec_search kvs_spec_check_uint16.
+  switcher kvs kvs_preamble kvs_spec_check_uint16 kvs_spec_addOrUpdate.
 
 Section KVS_spec_addOrUpdate_safe.
   Context
@@ -20,329 +20,6 @@ Section KVS_spec_addOrUpdate_safe.
   .
 
   (*** Specification from unknown *)
-  Lemma KVS_addOrupdate_spec_safe_pre
-    (Wca W : WORLD) (C : CmptName)
-    (pc_b pc_e pc_a : Addr)
-    (cgp_b cgp_e : Addr)
-    (wret wca0 wca1 wca2 : Word)
-    (m : kvs_map) (s : kvs_alloc)
-    ( E : coPset )
-    :
-
-    ↑Nkvs_otype ⊆ E ->
-
-    SubBounds pc_b pc_e pc_a (pc_a ^+ length kvs_addOrUpdate_instrs)%a ->
-    (cgp_b + length kvs_data)%a = Some cgp_e ->
-
-    related_sts_priv_world Wca W ->
-
-    ( (* initial register file *)
-      na_own cerise_nais E ∗
-      PC ↦ᵣ WCap RX Global pc_b pc_e pc_a ∗
-      cgp ↦ᵣ WCap RW Global cgp_b cgp_e cgp_b ∗
-      cra ↦ᵣ wret ∗
-      ca0 ↦ᵣ wca0 ∗ interp Wca C wca0 ∗ (* Sealed User Key *)
-      ca1 ↦ᵣ wca1 ∗ (* Key to update *)
-      ca2 ↦ᵣ wca2 ∗ interp Wca C wca2 ∗ (* New value *)
-      ctp ↦ᵣ - ∗ (* scratch *)
-      ct1 ↦ᵣ - ∗ (* scratch *)
-      ct2 ↦ᵣ - ∗ (* scratch *)
-      cnull ↦ᵣ - ∗
-
-      (* initial memory layout *)
-      codefrag pc_a kvs_addOrUpdate_instrs ∗
-      (pc_b ^+ UNSEALING_USER_KEY_OFFSET)%a ↦ₐ kvs_service_unsealing_key ∗
-
-      ▷ isKVS cgp_b m s ∗
-      ▷ seal_pred KVS_OTYPE kvs_otype_propC ∗
-
-      world_interp W C ∗
-
-      ▷ (na_own cerise_nais E ∗
-         PC ↦ᵣ updatePcPerm wret ∗
-         cgp ↦ᵣ - ∗
-         cra ↦ᵣ - ∗
-         ca1 ↦ᵣ WInt 0 ∗
-         ca2 ↦ᵣ - ∗
-         ctp ↦ᵣ - ∗ (* scratch *)
-         ct1 ↦ᵣ - ∗ (* scratch *)
-         ct2 ↦ᵣ - ∗ (* scratch *)
-         cnull ↦ᵣ - ∗
-
-         codefrag pc_a kvs_addOrUpdate_instrs ∗
-         (pc_b ^+ UNSEALING_USER_KEY_OFFSET)%a ↦ₐ kvs_service_unsealing_key ∗
-         (
-           (* THERE IS AN EMPTY SLOT AVAILABLE*)
-           (∃ idx (k : Z*Z) w,
-               (ca0 ↦ᵣ WInt ASM_TRUE ∗ isKVS cgp_b (<[idx := Some (kvs_full_key k.1 k.2, w)]> m) s))
-           ∨
-             (* THERE IS AN EMPTY SLOT AVAILABLE *)
-             (∃ idx (k : Z*Z) w,
-                 ca0 ↦ᵣ WInt ASM_TRUE ∗
-                 isKVS cgp_b (<[ idx := Some (kvs_full_key k.1 k.2, w)]> m) (kvs_alloc_insert s k.1 {[k.2]} ) )
-           ∨
-             (* THERE IS NO EMPTY SLOT AVAILABLE *)
-             (ca0 ↦ᵣ WInt ASM_FALSE ∗ isKVS cgp_b m s)
-         ) ∗
-
-         world_interp W C
-
-         -∗ WP Seq (Instr Executable) {{ v, ⌜v = HaltedV⌝ → na_own cerise_nais ⊤ }}
-        )
-      ⊢ WP Seq (Instr Executable) {{ v, ⌜v = HaltedV⌝ → na_own cerise_nais ⊤ }})%I.
-  Proof.
-    iIntros (HN HsubBounds Hcgp_contiguous Hrelated_Wca_W)
-      "(Hna & HPC & Hcgp & Hcra & Hca0 & Hinterp_wca0 & Hca1 & Hca2 & #Hinterp_wca2 & Hctp & Hct1 & Hct2 & [%wcnull Hcnull] &
-        Hcode & Ha_unsealing & HKVS & #Hspred & Hworld & Hpost)".
-    codefrag_facts "Hcode"; rename H into Hpc_contiguous ; clear H0.
-
-    (* --------------------------------------------------- *)
-    (* ----------------- Start the proof ----------------- *)
-    (* --------------------------------------------------- *)
-    rewrite /kvs_addOrUpdate_instrs /assembled_kvs_addOrUpdate.
-    rewrite -/(kvs_getFullKey ctp ca0 ca1 ct1 ct2).
-    rewrite -/(kvs_search ca0 ctp ct1 ct2).
-    rewrite -/(kvs_check_uint16 ca1 ct1).
-
-    focus_block_0 "Hcode" as "Hcode" "Hcont"; iHide "Hcont" as hcont.
-    iApply (KVS_check_uint16_spec with "[- $HPC $Hca1 $Hct1 $Hcode]"); eauto;iNext.
-    iIntros (nkey) "(-> & HPC & Hca1 & Hcode & Hct1)".
-    subst hcont; unfocus_block "Hcode" "Hcont" as "Hcode".
-
-    focus_block 1 "Hcode" as a_check_uint Ha_check_uint "Hcode" "Hcont"; iHide "Hcont" as hcont.
-    iDestruct "Hct1" as "[ (Hct1 & %Hnkey_uint16) | (Hct1 & %Hnkey_uint16)]"; cycle 1.
-    {
-      (* jnz (".addOrUpdate_not_uint16")%asm ct1; *)
-      iInstr "Hcode".
-      (* mov ca0 ASM_FALSE; *)
-      iInstr "Hcode".
-      (* mov ca1 0; *)
-      iInstr "Hcode".
-      (* jalr cnull cra; *)
-      iInstr "Hcode".
-      subst hcont; unfocus_block "Hcode" "Hcont" as "Hcode".
-      destruct (decide (ca0 = cnull)) as [|_]; first done.
-      iApply "Hpost"; iFrame.
-      iRight;iRight;iFrame.
-    }
-    (* jnz (".addOrUpdate_not_uint16")%asm ct1; *)
-    iInstr "Hcode".
-    (* jmp (".addOrUpdate_uint16_check_pass")%asm; *)
-    iInstr "Hcode".
-    subst hcont; unfocus_block "Hcode" "Hcont" as "Hcode".
-
-    focus_block 2 "Hcode" as a_get_full_key Ha_get_full_key "Hcode" "Hcont"; iHide "Hcont" as hcont
-    ; clear dependent Ha_check_uint.
-
-    iApply (KVS_getFullKey_spec_safe with
-             "[- $HPC $Hctp $Hca0 $Hinterp_wca0 $Hca1 $Hct1 $Hct2 $Ha_unsealing $Hcode $Hspred $Hworld]")
-    ; eauto; iNext.
-    iIntros (s' l_user_key user_key_addr user_key)
-      "(-> & %Hbounds_uk & %Hbounds_a_user_key & HPC & Hctp & Hca0 & Hca1 & Hct1 & Hct2
-      & Ha_unsealing & Hcode & Ha_user_key & Hres_open & Halloc & Hkvs_frags & Hworld)".
-    subst hcont; unfocus_block "Hcode" "Hcont" as "Hcode".
-
-    focus_block 3 "Hcode" as a_lea Ha_lea "Hcode" "Hcont"; iHide "Hcont" as hcont ; clear dependent Ha_get_full_key.
-    iInstr "Hcode" with "Hlc".
-    subst hcont; unfocus_block "Hcode" "Hcont" as "Hcode".
-
-    focus_block 4 "Hcode" as a_search Ha_search "Hcode" "Hcont"; iHide "Hcont" as hcont; clear dependent Ha_lea.
-    assert ( wf_kvs_full_key user_key nkey) as Hwk_fkey by (split; auto; lia).
-
-    destruct ( decide ( nkey ∈ s' ) ) as [Hfkey_in_s|Hfkey_notin_s].
-    (* The key has already been allocated *)
-    - iDestruct (big_sepS_elem_of_acc with "Hkvs_frags")
-        as "[ [%w [ [%idx Hkvs_frag] Hinterp_w] ] Hkvs_frags]"
-      ; eauto; iEval (cbn) in "Hkvs_frag".
-      iApply (KVS_search_spec_in with "[- $HPC $Hcgp $Hca0 $Hctp $Hct1 $Hct2 $HKVS $Hkvs_frag $Hcode]"); eauto.
-      { rewrite /withinBounds; solve_addr. }
-      iNext; iIntros "(HPC & Hcgp & Hca0 & Hctp & Hct1 & Hct2 & HKVS & Hcgp_opt & Hcgp_key & Hcgp_val & Hkvs_frag & %Hcgp_idx & Hcode)".
-      iDestruct (isKVS_open_valid with "HKVS Hkvs_frag") as "%Hm_idx".
-      iDestruct (isKVS_open_indom_idx with "HKVS") as "%Hidx".
-      { by apply elem_of_dom_2 in Hm_idx. }
-      subst hcont; unfocus_block "Hcode" "Hcont" as "Hcode".
-
-      focus_block 5 "Hcode" as a_addOrUpdate Ha_addOrUpdate "Hcode" "Hcont"; iHide "Hcont" as hcont; clear dependent Ha_search.
-      (* Sub ctp ct1 (-1) *)
-      iInstr "Hcode".
-      (* Jnz 5 ctp *)
-      iInstr "Hcode".
-      { injection; intros; lia. }
-      (* Lea cgp 2 *)
-      iInstr "Hcode".
-      { transitivity ( Some ((cgp_b ^+ (ASM_SIZEOF_KVS_ENTRY * idx + 2))%a) ); solve_addr+Hcgp_idx Hidx. }
-      (* Store cgp (inr ca2) *)
-      destruct (canStore RW wca2) eqn:HcanStore_wca2; cycle 1.
-      {
-       iInstr_lookup "Hcode" as "Hi" "Hcode".
-        wp_instr.
-        iApply (rules_Store.wp_store_fail_reg_perm with "[$HPC $Hi $Hca2 $Hcgp]"); try solve_pure.
-        iNext; iIntros "_".
-        wp_pure; wp_end; iIntros "%Hcontr";done.
-      }
-      iInstr_lookup "Hcode" as "Hi" "Hcode".
-      wp_instr.
-      iApply (rules_Store.wp_store_success_reg with "[$HPC $Hi $Hca2 $Hcgp $Hcgp_val]"); try solve_pure.
-      iNext; iIntros "(HPC & Hi & Hca2 & Hcgp & Hcgp_val)".
-      wp_pure.
-      iInstr_close "Hcode".
-
-      (* Mov ca0 0 *)
-      iInstr "Hcode".
-      (* Mov ca1 0 *)
-      iInstr "Hcode".
-      (* Jalr cnull cra *)
-      iInstr "Hcode".
-      subst hcont; unfocus_block "Hcode" "Hcont" as "Hcode".
-
-      iMod (isKVS_open_update _ _ _ idx (kvs_full_key user_key nkey) _ wca2 with "HKVS Hkvs_frag") as "[HKVS Hkvs_frag]".
-
-      iDestruct (close_isKVS with "[$HKVS Hcgp_opt Hcgp_key Hcgp_val]") as "HKVS";eauto.
-      { by simplify_map_eq. }
-      { iFrame. }
-
-      iDestruct ("Hkvs_frags" with "[$Hkvs_frag]") as "Hkvs_frags"; eauto.
-      { cbn ; iIntros (W' Hrelated_W_W').
-        iApply (monotone.interp_monotone_nl with "[] [] [$Hinterp_wca2]"); iPureIntro.
-        + eapply related_sts_priv_trans_world; eauto.
-        + eapply (canStore_global_nonisWL RW); done.
-      }
-
-      iAssert (kvs_otype_propC (W, C, (force_global (WSealable (kvs_user_seal_key_scap l_user_key user_key_addr)))))
-        with "[Ha_user_key Halloc Hkvs_frags]"
-        as "HP".
-      { iExists user_key, user_key_addr, s'; iFrame "∗ %".
-        iPureIntro; auto.
-      }
-      iDestruct (sclose_world_interp_singleton with "Hspred Hres_open HP Hworld") as "Hworld".
-
-      iApply "Hpost"; iFrame "Hna HPC Hcgp Hcra Hctp Hct1 Hct2 Hca1 Hca2 Hcnull Hcode Ha_unsealing Hworld".
-      iLeft; iExists idx, (user_key, nkey), wca2; iFrame.
-
-    (* The key has never been allocated *)
-    - iApply (KVS_search_spec_empty_slot with "[- $HPC $Hcgp $Hca0 $Hctp $Hct1 $Hct2 $HKVS $Halloc $Hcode]"); eauto.
-      { rewrite /withinBounds; solve_addr. }
-      iNext; iIntros "[
-      (%idx_empty & HPC & Hcgp & Hca0 & Hctp & Hct1 & Hct2 & Halloc & HKVS
-      & Hcgp_opt & [%wkey Hcgp_key] & [%wval Hcgp_val] & Hfkey & %Hcgp_bounds & %Hidx_empty & Hcode)
-      | (HPC & Hcgp & Hca0 & Hctp & Hct1 & Hct2 & Halloc & HKVS & Hcode) ]".
-      all: subst hcont; unfocus_block "Hcode" "Hcont" as "Hcode".
-      + (* An empty slot was found *)
-
-        focus_block 5 "Hcode" as a_addOrUpdate Ha_addOrUpdate "Hcode" "Hcont"; iHide "Hcont" as hcont; clear dependent Ha_search.
-        (* sub ctp ctp (-1)%Z; *)
-        iInstr "Hcode".
-        replace (-1 - -1)%Z with 0%Z by lia.
-        (* jnz (".addOrUpdate_key_found")%asm ctp; *)
-        iInstr "Hcode".
-        (* sub ctp ct1 (-1)%Z; *)
-        iInstr "Hcode".
-        (* jnz (".addOrUpdate_empty_slot_found")%asm ctp; *)
-        iInstr "Hcode".
-        { intro; simplify_eq; lia. }
-        (* mul ct1 ct1 ASM_SIZEOF_KVS_ENTRY *)
-        iInstr "Hcode".
-        (* lea cgp ct1; *)
-        iInstr "Hcode".
-        { transitivity (Some (cgp_b ^+ ASM_SIZEOF_KVS_ENTRY * idx_empty)%a); solve_addr+ Hidx_empty Hcgp_bounds. }
-        (* store cgp ASM_SOME; *)
-        iInstr "Hcode".
-        { solve_addr+Hcgp_bounds. }
-        (* lea cgp 1; *)
-        iInstr "Hcode".
-        { transitivity (Some (cgp_b ^+ (ASM_SIZEOF_KVS_ENTRY * idx_empty + 1))%a); solve_addr+ Hidx_empty Hcgp_bounds. }
-        (* store cgp ca0; *)
-        iInstr_lookup "Hcode" as "Hi" "Hcode".
-        wp_instr.
-        iApply (rules_Store.wp_store_success_reg with "[$HPC $Hi $Hca0 $Hcgp $Hcgp_key]"); try solve_pure.
-        { solve_addr+Hcgp_bounds. }
-        { done. }
-        iNext; iIntros "(HPC & Hi & Hca0 & Hcgp & Hcgp_key)".
-        wp_pure.
-        iInstr_close "Hcode".
-        (* lea cgp 1; *)
-        iInstr "Hcode".
-        { transitivity (Some (cgp_b ^+ (ASM_SIZEOF_KVS_ENTRY * idx_empty + 2))%a); solve_addr+ Hidx_empty Hcgp_bounds. }
-        (* store cgp ca2; *)
-        destruct (canStore RW wca2) eqn:HcanStore_wca2; cycle 1.
-        {
-          iInstr_lookup "Hcode" as "Hi" "Hcode".
-          wp_instr.
-          iApply (rules_Store.wp_store_fail_reg_perm with "[$HPC $Hi $Hca2 $Hcgp]"); try solve_pure.
-          iNext; iIntros "_".
-          wp_pure; wp_end; iIntros "%Hcontr";done.
-        }
-        iInstr_lookup "Hcode" as "Hi" "Hcode".
-        wp_instr.
-        iApply (rules_Store.wp_store_success_reg with "[$HPC $Hi $Hca2 $Hcgp $Hcgp_val]"); try solve_pure.
-        iNext; iIntros "(HPC & Hi & Hca2 & Hcgp & Hcgp_val)".
-        wp_pure.
-        iInstr_close "Hcode".
-        (* mov ca0 ASM_TRUE; *)
-        iInstr "Hcode".
-        (* mov ca1 0; *)
-        iInstr "Hcode".
-        (* jalr cnull cra; *)
-        iInstr "Hcode".
-        subst hcont; unfocus_block "Hcode" "Hcont" as "Hcode".
-
-        iMod (isKVS_open_insert _ _ _ _ _ _ _ wca2 with "HKVS Halloc Hfkey") as "(HKVS & Halloc & Hfkey)"; eauto.
-        iDestruct (close_isKVS with "[$HKVS Hcgp_opt Hcgp_key Hcgp_val]") as "HKVS";eauto.
-        { by simplify_map_eq. }
-        { iFrame. }
-
-        iDestruct ( big_sepS_insert with "[$Hkvs_frags Hfkey]") as "Hkvs_frags";eauto.
-        { iExists wca2; iFrame.
-          cbn; iIntros (W' Hrelated_W_W').
-          iApply (monotone.interp_monotone_nl with "[] [] [$Hinterp_wca2]"); iPureIntro.
-          + eapply related_sts_priv_trans_world; eauto.
-          + eapply (canStore_global_nonisWL RW); done.
-        }
-
-
-        iAssert (kvs_otype_propC (W, C, (force_global (WSealable (kvs_user_seal_key_scap l_user_key user_key_addr)))))
-        with "[Ha_user_key Halloc Hkvs_frags]"
-        as "HP".
-        { iExists user_key, user_key_addr, ({[nkey]} ∪ s'); iFrame "∗ %".
-          iPureIntro; auto.
-        }
-        iDestruct (sclose_world_interp_singleton with "Hspred Hres_open HP Hworld") as "Hworld".
-
-        iApply "Hpost"; iFrame "Hna HPC Hcgp Hcra Hctp Hct1 Hct2 Hca1 Hca2 Hcnull Hcode Ha_unsealing Hworld".
-        iRight; iLeft; iExists idx_empty, (user_key, nkey), wca2; iFrame.
-
-      + (* No empty slot found *)
-        focus_block 5 "Hcode" as a_addOrUpdate Ha_addOrUpdate "Hcode" "Hcont"; iHide "Hcont" as hcont; clear dependent Ha_search.
-        (* sub ct1 ct1 (-1)%Z; *)
-        iInstr "Hcode".
-        replace (-1 - -1)%Z with 0%Z by lia.
-        (* jnz (".addOrUpdate_key_found")%asm ctp; *)
-        iInstr "Hcode".
-        (* sub ct1 ct1 (-1)%Z; *)
-        iInstr "Hcode".
-        replace (-1 - -1)%Z with 0%Z by lia.
-        (* jnz (".addOrUpdate_empty_slot_found")%asm ct1; *)
-        iInstr "Hcode".
-        (* mov ca0 ASM_FALSE; *)
-        iInstr "Hcode".
-        (* mov ca1 0; *)
-        iInstr "Hcode".
-        (* jalr cnull cra; *)
-        iInstr "Hcode".
-        subst hcont; unfocus_block "Hcode" "Hcont" as "Hcode".
-
-        iAssert (kvs_otype_propC (W, C, (force_global (WSealable (kvs_user_seal_key_scap l_user_key user_key_addr)))))
-        with "[Ha_user_key Halloc Hkvs_frags]"
-        as "HP".
-        { iExists user_key, user_key_addr, s'; iFrame "∗ %".
-          iPureIntro; auto.
-        }
-        iDestruct (sclose_world_interp_singleton with "Hspred Hres_open HP Hworld") as "Hworld".
-
-        iApply "Hpost"; iFrame "Hna HPC Hcgp Hcra Hctp Hct1 Hct2 Hca1 Hca2 Hcnull Hcode Ha_unsealing Hworld".
-        iRight; iRight; iFrame.
-  Qed.
-
   Lemma KVS_addOrupdate_spec_safe
     (Wca W : WORLD) (C : CmptName)
     (wret wca0 wca1 wca2 : Word)
@@ -390,10 +67,10 @@ Section KVS_spec_addOrUpdate_safe.
       ⊢ WP Seq (Instr Executable) {{ v, ⌜v = HaltedV⌝ → na_own cerise_nais ⊤ }})%I.
   Proof.
     iIntros (Hnkvs_E Hnkvs_otype_E Hrelated_Wca_W)
-      "(#Hkvs_inv & Hna & HPC & Hcgp & Hcra & Hca0 & Hinterp_ca0
-      & Hca1 & Hca2 & Hinterp_ca2 & Hctp & Hct1 & Hct2 & Hcnull & Hworld & Hpost)".
+      "(#Hkvs_inv & Hna & HPC & Hcgp & Hcra & Hca0 & #Hinterp_wca0
+      & Hca1 & Hca2 & #Hinterp_wca2 & Hctp & Hct1 & Hct2 & Hcnull & Hworld & Hpost)".
     iMod (na_inv_acc with "Hkvs_inv Hna")
-      as "( (%m & %s & >Himports & >Hcode & HisKVS & #Hspred) & Hna & Hkvs_inv_close)"; eauto.
+      as "( (%m & %s & >Himports & >Hcode & HKVS & #Hspred) & Hna & Hkvs_inv_close)"; eauto.
     pose proof (Hcgp_continuous := KVS_size_data).
     pose proof (HKVS_pcc_b' := KVS_size_imports).
     pose proof (Hcode_continuous := KVS_size_code).
@@ -411,21 +88,130 @@ Section KVS_spec_addOrUpdate_safe.
     focus_block_0 "Hcode" as "Hcode" "Hcont"; iHide "Hcont" as hcont.
     assert (kvs_addOrUpdate_pcc_addr = KVS_pcc_b')
       as -> by (rewrite /kvs_addOrUpdate_pcc_addr /kvs_addOrUpdate_pcc_off; solve_addr+HKVS_pcc_b').
-    iApply (KVS_addOrupdate_spec_safe_pre _ _ _ _ _ _ _ _ _ wca0 with "[- $HPC]"); last iFrame "∗#"; eauto.
-    { pose proof Nkvs_namespaces_disjoint as (?&?&?); solve_ndisj. }
 
-    iNext; iIntros "(Hna & HPC & Hcgp & Hcra & Hca1 & Hca2 & Hctp & Hct1 & Hct2
-              & Hcnull & Hcode & Ha_unsealing & HKVS & Hworld)".
-    subst hcont; unfocus_block "Hcode" "Hcont" as "Hcode".
+    (* Destruct validity map key *)
+    destruct (decide (word_is_uint16 wca1)) as [Hwca1_uint16|Hwca1_uint16]; cycle 1.
+    { (* the map key argument is not a uint16 *)
+      iApply KVS_addOrUpdate_spec_not_uint16_map_key; eauto; iFrame.
+      iNext; iIntros "(HPC & Hcra & Hca0 & Hca1 & Hct1 & Hcnull & Hcode)".
+      subst hcont; unfocus_block "Hcode" "Hcont" as "Hcode".
+      iMod ("Hkvs_inv_close" with "[$Hna $Hcode Himports_sw Ha_unsealing $HKVS $Hspred]") as "Hna"
+      ; last ( iApply "Hpost"; iFrame); try (iLeft; iFrame).
+      iApply (region_pointsto_cons with "[Ha_unsealing Himports_sw]"); eauto; iFrame.
+      iApply (region_pointsto_cons with "[Ha_unsealing]"); eauto; [solve_addr+|]; iFrame.
+      rewrite /region_pointsto finz_seq_between_empty; auto; solve_addr+.
+    }
+    destruct wca1 as [nkey| | | ]; cbn in Hwca1_uint16; try done.
 
-    iDestruct "HKVS" as
-      "[ (%idx & %k & %w & Hca0 & HKVS) | [ (%idx & %k & %w & Hca0 & HKVS) | (Hca0 & HKVS) ] ]".
-    all: iMod ("Hkvs_inv_close" with "[$Hna $Hcode Himports_sw Ha_unsealing $HKVS $Hspred]") as "Hna"
-    ; auto; last ( iApply "Hpost"; iFrame ; try (iLeft; iFrame; done) ; try (iRight; iFrame; done)).
-    all: iNext.
-    all: iApply (region_pointsto_cons with "[Ha_unsealing Himports_sw]"); eauto; iFrame.
-    all: iApply (region_pointsto_cons with "[Ha_unsealing]"); eauto; [solve_addr+|]; iFrame.
-    all: rewrite /region_pointsto finz_seq_between_empty; auto; solve_addr+.
+    (* Destruct validity user key *)
+    destruct ( is_sealed_with_o wca0 KVS_OTYPE ) eqn:Hwca0_sealed_with_kvs_ot; cycle 1.
+    { (* the user key argument is not a valid sealed user key *)
+      iApply KVS_addOrUpdate_spec_invalid_sealed_user_key; eauto; iFrame.
+    }
+    (* The inputs are valid. *)
+    rewrite /is_sealed_with_o in Hwca0_sealed_with_kvs_ot.
+    destruct wca0 as [ | | | ot wsb ]; try done.
+    rewrite Z.eqb_eq in Hwca0_sealed_with_kvs_ot.
+    assert (ot = KVS_OTYPE) by solve_addr+Hwca0_sealed_with_kvs_ot; simplify_eq.
+
+    (* Open sealing predicate of sealed user key *)
+    iDestruct (monotone.interp_monotone_sd with "[] Hinterp_wca0") as "Hinterp_wca0_W"; auto.
+    iEval (rewrite fixpoint_interp1_eq /= /interp_sb) in "Hinterp_wca0".
+    iAssert (▷ sts_seals_std C KVS_OTYPE {[WSealable wsb]})%I as "#Hinterp_wca0'".
+    { iApply sts_seals_std_weaken; last iFrame "Hinterp_wca0"; last set_solver+. }
+    iAssert (▷ world_interp W C)%I with "Hworld" as "Hworld".
+
+    iDestruct (sopen_world_interp_singleton with "Hspred Hinterp_wca0' Hworld")
+                as "(Hworld & Hres_open & HP)".
+    rewrite /kvs_otype_propC /= /kvs_otype_prop //= /kvs_otype_inv.
+    iDestruct "HP" as "(%ku & %a & %s' & Heq_sb & Hku & Hbounds & Ha & Halloc & Hfkeys)".
+
+    (* Either the map key is already allocated, or it is not *)
+    destruct ( decide (nkey ∈ s') ) as [Hs' | Hs'].
+    - iDestruct (big_sepS_elem_of_acc with "Hfkeys")
+        as "[ [%w [ [%idx Hkvs_frag] #Hinterp_w] ] Hfkeys]"
+      ; eauto; iEval (cbn) in "Hkvs_frag".
+      iApply KVS_update_spec_pre_gen; last iFrame; eauto.
+      iNext; iNext.
+      iIntros "(%Heq_sb & %Hku & %Hbounds & %Hcan_store
+                & HPC & Hgcp & Hcra & Hca0 & Hca1 & Hca2 & Hctp & Hct1 & Hct2 & Hcnull
+                & HKVS & Hkvs_frag & Hcode & Ha_unsealing & Ha)".
+      subst hcont; unfocus_block "Hcode" "Hcont" as "Hcode".
+
+      destruct wsb as [ ? l_user_key ? ? ? | ]; cbn in Hbounds; simplify_eq.
+      iDestruct ("Hfkeys" with "[$Hkvs_frag Hinterp_wca2]") as "Hfkeys".
+      { cbn ; iIntros (W' Hrelated_W_W').
+        iApply (monotone.interp_monotone_nl with "[] [] [$Hinterp_wca2]"); iPureIntro.
+        + eapply related_sts_priv_trans_world; eauto.
+        + eapply (canStore_global_nonisWL RW); done.
+      }
+
+      iAssert (kvs_otype_propC (W, C, (force_global (WSealable (kvs_user_seal_key_scap l_user_key a)))))
+        with "[Ha Halloc Hfkeys]"
+        as "HP".
+      { iFrame "∗%#"; iPureIntro; auto. }
+      iDestruct (sclose_world_interp_singleton with "Hspred Hres_open HP Hworld") as "Hworld".
+
+      iMod ("Hkvs_inv_close" with "[$Hna $Hcode Himports_sw Ha_unsealing $HKVS $Hspred]") as "Hna".
+      {
+        iNext.
+        iApply (region_pointsto_cons with "[Ha_unsealing Himports_sw]"); eauto; iFrame.
+        iApply (region_pointsto_cons with "[Ha_unsealing]"); eauto; [solve_addr+|]; iFrame.
+        rewrite /region_pointsto finz_seq_between_empty; auto; solve_addr+.
+      }
+      iApply "Hpost"; iFrame.
+
+    - iApply KVS_add_spec_pre_gen; last iFrame; eauto.
+      iNext; iNext.
+      iIntros "(%Heq_sb & %Hku & %Hbounds
+                & HPC & Hgcp & Hcra & Hca1 & Hca2 & Hctp & Hct1 & Hct2 & Hcnull
+                & Hcode & Ha_unsealing & Ha
+                & Hrest)".
+      subst hcont; unfocus_block "Hcode" "Hcont" as "Hcode".
+      destruct wsb as [ ? l_user_key ? ? ? | ]; cbn in Hbounds; simplify_eq.
+
+
+      iDestruct "Hrest" as
+        "[ (%idx & %Hcan_store & Hca0 & HKVS & Halloc & Hkvs_frag)
+                  | (Hca0 & HKVS & Halloc)
+                  ]".
+      + iDestruct ( big_sepS_insert with "[Hkvs_frag $Hfkeys]") as "Hfkeys";eauto.
+        { iExists wca2; iFrame.
+          cbn; iIntros (W' Hrelated_W_W').
+          iApply (monotone.interp_monotone_nl with "[] [] [$Hinterp_wca2]"); iPureIntro.
+          + eapply related_sts_priv_trans_world; eauto.
+          + eapply (canStore_global_nonisWL RW); done.
+        }
+
+        iAssert (kvs_otype_propC (W, C, (force_global (WSealable (kvs_user_seal_key_scap l_user_key a)))))
+          with "[Ha Halloc Hfkeys]"
+          as "HP".
+        { iFrame "∗%"; iPureIntro; auto. }
+        iDestruct (sclose_world_interp_singleton with "Hspred Hres_open HP Hworld") as "Hworld".
+
+        iMod ("Hkvs_inv_close" with "[$Hna $Hcode Himports_sw Ha_unsealing $HKVS $Hspred]") as "Hna".
+        {
+          iNext.
+          iApply (region_pointsto_cons with "[Ha_unsealing Himports_sw]"); eauto; iFrame.
+          iApply (region_pointsto_cons with "[Ha_unsealing]"); eauto; [solve_addr+|]; iFrame.
+          rewrite /region_pointsto finz_seq_between_empty; auto; solve_addr+.
+        }
+        iApply "Hpost"; iFrame.
+
+      + iAssert (kvs_otype_propC (W, C, (force_global (WSealable (kvs_user_seal_key_scap l_user_key a)))))
+          with "[Ha Halloc Hfkeys]"
+          as "HP".
+        { iFrame "∗%"; iPureIntro; auto. }
+        iDestruct (sclose_world_interp_singleton with "Hspred Hres_open HP Hworld") as "Hworld".
+
+        iMod ("Hkvs_inv_close" with "[$Hna $Hcode Himports_sw Ha_unsealing $HKVS $Hspred]") as "Hna".
+        {
+          iNext.
+          iApply (region_pointsto_cons with "[Ha_unsealing Himports_sw]"); eauto; iFrame.
+          iApply (region_pointsto_cons with "[Ha_unsealing]"); eauto; [solve_addr+|]; iFrame.
+          rewrite /region_pointsto finz_seq_between_empty; auto; solve_addr+.
+        }
+        iApply "Hpost"; iFrame.
   Qed.
 
 
